\documentclass[10pt]{report}
\usepackage[spanish,activeacute]{babel}
\usepackage{caption}
\usepackage{subcaption}
\usepackage[latin1]{inputenc}
\usepackage{babel}
\usepackage{picture}
\usepackage{url}
\usepackage{mathrsfs}
\usepackage{amssymb,amsthm,amsmath,latexsym}
\usepackage[round]{natbib}
\usepackage{fancyhdr}
\theoremstyle{plain}
\newtheorem{teo}{Teorema}
\newtheorem{prop}[teo]{Proposicion}
\newtheorem{defi}[teo]{Definicion}
\newtheorem{obs}[teo]{Observacion}
\newtheorem{lem}[teo]{Lema}
\newtheorem{cor}[teo]{Corolario}
\usepackage[pdftex]{color,graphicx}
\newcommand{\sgn}{\mathop{\mathrm{sgn}}}
\begin{document}
\chapter{Verosimilitudes Extendidas}
\section{$\pi(\alpha_d|(\theta_{ij})_{j=1}^{n_i}._{i=1}^I)$}
\begin{eqnarray*}
\pi(\alpha_d|(\theta_{ij})_{j=1}^{n_i}._{i=1}^I) &\propto& \Big(\prod_{i=1}^I Gamma(\theta_{i1}|\alpha_d+\alpha_\theta, d_{i1}+\beta_\theta \times \prod_{i=1}^I \prod_{j=2}^{n_i} Gamma(\theta_{ij}|2\alpha_d+\alpha_\theta, d_{ij}+d_{ij-1}+\beta_\theta) \Big) \\
&\times& Gamma(\alpha_d|\alpha_0,\beta_0)\\
\end{eqnarray*}

\begin{eqnarray*}
&=& \bigg(\prod_{i=1}^I \frac{(d_{i1}+\beta_\theta)^{\alpha_d+\alpha_\theta}}{\Gamma(\alpha_d+\alpha_\theta)} \quad \theta_{i1}^{\alpha_d+\alpha_\theta} e^{-\theta_{i1}(d_{i1}+\beta_\theta)} \\
&\times& \prod_{i=1}^I \prod_{j=2}^{n_i} \frac{(d_{ij}+d_{ij-1}+\beta_\theta)^{2\alpha_d+\alpha_\theta}}{\Gamma(2\alpha_d+\alpha_\theta)} \quad \theta_{ij}^{2\alpha_d+\alpha_\theta-1} e^{-\theta_{ij}(d_{ij}+d_{ij-1}+\beta_\theta)}\bigg)\\
&\times& \frac{\beta_0^{\alpha_0}}{\Gamma(\alpha_0)} \alpha_d^{\alpha_0-1} e^{-\alpha_d\beta_0}
\end{eqnarray*}

\begin{eqnarray*}
&\propto& \Big(\frac{1}{\Gamma(\alpha_d+\alpha_\theta)}\Big)^I \Big(\frac{1}{\Gamma(2\alpha_d+\alpha_\theta)}\Big)^{\sum_{i=1}^I n_i} \quad \alpha_d^{\alpha_0-1} e^{-\alpha_d\beta_0} \times \\
&\times& \Bigg(\prod_{i=1}^I (d_{i1}+\beta_\theta)^{\alpha_d+\alpha_\theta} \quad \theta_{i1}^{\alpha_d+\alpha_\theta-1} \prod_{i=1}^I \prod_{j=2}^{n_i} (d_{ij}+d_{ij-1}+\beta_\theta)^{2\alpha_d+\alpha_\theta}\quad \theta_{ij}^{2\alpha_d+\alpha_\theta-1}\Bigg)
\end{eqnarray*}
\\
\\
\section{$\pi(\alpha_\theta|(\theta_{ij})_{i=1}^I._{j=1}^{n_i})$}
\begin{eqnarray*}
\pi(\alpha_\theta|(\theta_{ij})_{j=1}^{n_i}._{i=1}^I) &\propto& \Big(\prod_{i=1}^I Gamma(\theta_{i1}|\alpha_d+\alpha_\theta, d_{i1}+\beta_\theta \times \prod_{i=1}^I \prod_{j=2}^{n_i} Gamma(\theta_{ij}|2\alpha_d+\alpha_\theta, d_{ij}+d_{ij-1}+\beta_\theta) \Big) \\
&\times& Gamma(\alpha_\theta|\alpha_0,\beta_0)\\
\end{eqnarray*}

\begin{eqnarray*}
&=&\Bigg(\prod_{i=1}^I \frac{(d_{i1}+\beta_\theta)^{\alpha_d+\alpha_\theta}}{\Gamma(\alpha_d+\alpha_\theta)} \quad \theta_{i1}^{\alpha_d+\alpha_\theta-1} e^{-\theta_{i1}(d_{i1}+\beta_\theta)} \times\\
&\times& \prod_{i=1}^I \prod_{j=2}^{n_i} \frac{(d_{ij}+d_{ij-1}+\beta_\theta)^{2\alpha_d+\alpha_\theta}}{\Gamma(2\alpha_d+\alpha_\theta)} \quad \theta_{ij}^{2\alpha_d+\alpha_\theta-1} e^{-\theta_{ij}(d_{ij}+d_{ij-1}+\beta_\theta)}\Bigg) \times \\
&\times & \frac{\beta_0^{\alpha_0}}{\Gamma(\alpha_0)} \quad \alpha_\theta^{\alpha_0-1} e^{-\alpha_\theta\beta_0}
\end{eqnarray*}
\\
\begin{eqnarray*}
&\propto& \Bigg(\prod_{i=1}^I \frac{(d_{i1}+\beta_\theta)^{\alpha_d+\alpha_\theta}}{\Gamma(\alpha_d+\alpha_\theta)} \quad \theta_{i1}^{\alpha_d+\alpha_\theta-1} \quad \prod_{i=1}^I \prod_{j=2}^{n_i} \frac{(d_{ij}+d_{ij-1}+\beta_\theta)^{2\alpha_d+\alpha_\theta}}{\Gamma(2\alpha_d+\alpha_\theta)}\quad\theta_{ij}^{2\alpha_d+\alpha_\theta-1}\Bigg) \times \alpha_\theta^{\alpha_0-1} \quad e^{-\alpha_\theta\beta_0}
\end{eqnarray*}
\\
\\
\begin{eqnarray*}
&=&\Big(\frac{1}{\Gamma(\alpha_d+\alpha_\theta)}\Big)^I \Big(\frac{1}{\Gamma(2\alpha_d+\alpha_\theta)}\Big)^{\sum_{i=1}^I n_i} \quad \alpha_\theta^{\alpha_0-1} e^{-\alpha_\theta\beta_0} \times \\
&\times& \Bigg(\prod_{i=1}^I (d_{i1}+\beta_\theta)^{\alpha_d+\alpha_\theta} \quad \theta_{i1}^{\alpha_d+\alpha_\theta-1}\quad \prod_{i=1}^I \prod_{j=2}^{n_i} (d_{ij}+d_{ij-1}+\beta_\theta)^{2\alpha_d+\alpha_\theta} \quad \theta_{ij}^{2\alpha_d+\alpha_\theta-1}\Bigg)
\end{eqnarray*}
\\
\\
\\
\section{$\pi(\beta_\theta|(\theta_{ij})_{i=1}^I._{j=1}^{n_i})$}
\begin{eqnarray*}
\pi(\beta_\theta|(\theta_{ij})_{j=1}^{n_i}._{i=1}^I) &\propto& \Big(\prod_{i=1}^I Gamma(\theta_{i1}|\alpha_d+\alpha_\theta, d_{i1}+\beta_\theta \times \prod_{i=1}^I \prod_{j=2}^{n_i} Gamma(\theta_{ij}|2\alpha_d+\alpha_\theta, d_{ij}+d_{ij-1}+\beta_\theta) \Big) \\
&\times& Gamma(\beta_\theta|\alpha_0,\beta_0)\\
\end{eqnarray*}
\\
\begin{eqnarray*}
&=&\Bigg(\prod_{i=1}^I \frac{(d_{i1}+\beta_\theta)^{\alpha_d+\alpha_\theta}}{\Gamma(\alpha_d+\alpha_\theta)} \quad \theta_{i1}^{\alpha_d+\alpha_\theta-1} e^{-\theta_{i1}(d_{i1}+\beta_\theta)} \times\\
&\times& \prod_{i=1}^I \prod_{j=2}^{n_i} \frac{(d_{ij}+d_{ij-1}+\beta_\theta)^{2\alpha_d+\alpha_\theta}}{\Gamma(2\alpha_d+\alpha_\theta)} \quad \theta_{ij}^{2\alpha_d+\alpha_\theta-1} e^{-\theta_{ij}(d_{ij}+d_{ij-1}+\beta_\theta)}\Bigg) \times \\
&\times & \frac{\beta_0^{\alpha_0}}{\Gamma(\alpha_0)} \quad \beta_\theta^{\alpha_0-1} e^{-\beta_\theta\beta_0}
\end{eqnarray*}
\\
\begin{eqnarray*}
&\propto& \Bigg(\prod_{i=1}^I (d_{i1}+\beta_\theta)^{\alpha_d+\alpha_\theta}\times \prod_{i=1}^I \prod_{j=2}^{n_i} (d_{ij}+d_{ij-1}+\beta_\theta)^{2\alpha_d+\alpha_\theta}\quad \Bigg)\times \beta_\theta^{\alpha_0-1} e^{-\beta_\theta\big(\beta_0+\sum_{i=1}^I \sum_{j=1}^{n_i}\theta_{ij}\big)}
\end{eqnarray*}
\\
\\
\\
\section{$\pi(\alpha_\gamma|(\gamma_{ij})_{i=1}^I._{j=1}^{n_i})$}
\begin{eqnarray*}
\pi(\alpha_\gamma|(\gamma_{ij})_{i=1}^I._{j=1}^{n_i}) &\propto& \Bigg(\prod_{i=1}^I \bigg(\frac{1}{\gamma_{i1}}\bigg)^{d_{i1+\alpha_\gamma+1}}\quad e^{-\big((\frac{\beta_\gamma}{\gamma_{i1}})+(\frac{c_{i1}}{\gamma_{i1}})^{d_{i1}}\big)}\times\\
&\times& \prod_{i=1}^I \prod_{j=2}^{n_i} \bigg(\frac{1}{\gamma_{ij}}\bigg)^{2d_{ij}+\alpha_\gamma+1}\quad e^{-\big((\frac{\beta_\gamma}{\gamma_{ij}})+(\frac{c_{ij}+c_{ij-1}}{\gamma_{ij}})^{d_{ij}}\big)}\Bigg)\times \\
&\times& Gamma(\alpha_\gamma|\alpha_0,\beta_0)
\end{eqnarray*}
\\
\begin{eqnarray*}
&=&\Bigg(\prod_{i=1}^I \bigg(\frac{1}{\gamma_{i1}}\bigg)^{d_{i1+\alpha_\gamma+1}}\quad e^{-\big((\frac{\beta_\gamma}{\gamma_{i1}})+(\frac{c_{i1}}{\gamma_{i1}})^{d_{i1}}\big)}\times\\
&\times& \prod_{i=1}^I \prod_{j=2}^{n_i} \bigg(\frac{1}{\gamma_{ij}}\bigg)^{2d_{ij}+\alpha_\gamma+1}\quad e^{-\big((\frac{\beta_\gamma}{\gamma_{ij}})+(\frac{c_{ij}+c_{ij-1}}{\gamma_{ij}})^{d_{ij}}\big)}\Bigg)\times \\
&\times& \frac{\beta_0^{\alpha_0}}{\Gamma(\alpha_0)} \quad \alpha_\gamma^{\alpha_0-1} e^{-\alpha_\gamma\beta_0}
\end{eqnarray*}
\\
\\
\begin{eqnarray*}
&\propto& \Bigg(\prod_{i=1}^I \Big(\frac{1}{\gamma_{i1}}\Big)^{\alpha_\gamma} \times \prod_{i=1}^I \prod_{j=2}^{n_i}\Big(\frac{1}{\gamma_{ij}}\Big)^{\alpha_\gamma}\Bigg)\quad \alpha_\gamma^{\alpha_0-1}e^{-\alpha_\gamma\beta_0}
\end{eqnarray*}
\\
\begin{eqnarray*}
&=&\Bigg(\prod_{i=1}^I \prod_{j=1}^{n_i} \Big(\frac{1}{\gamma_{ij}}\Big)^{\alpha_\gamma}\Bigg) \quad \alpha_\gamma^{\alpha_0-1}e^{-\alpha_\gamma\beta_0}
\end{eqnarray*}
\\
\\
\\
\section{$\pi(\beta_\gamma|(\gamma_{ij})_{i=1}^I._{j=1}^{n_i})$}
\begin{eqnarray*}
\pi(\alpha_\gamma|(\gamma_{ij})_{i=1}^I._{j=1}^{n_i}) &\propto& \Bigg(\prod_{i=1}^I \bigg(\frac{1}{\gamma_{i1}}\bigg)^{d_{i1+\alpha_\gamma+1}}\quad e^{-\big((\frac{\beta_\gamma}{\gamma_{i1}})+(\frac{c_{i1}}{\gamma_{i1}})^{d_{i1}}\big)}\times\\
&\times& \prod_{i=1}^I \prod_{j=2}^{n_i} \bigg(\frac{1}{\gamma_{ij}}\bigg)^{2d_{ij}+\alpha_\gamma+1}\quad e^{-\big((\frac{\beta_\gamma}{\gamma_{ij}})+(\frac{c_{ij}+c_{ij-1}}{\gamma_{ij}})^{d_{ij}}\big)}\Bigg)\times \\
&\times& Gamma(\beta_\gamma|\alpha_0,\beta_0)
\end{eqnarray*}
\\
\begin{eqnarray*}
&=&\Bigg(\prod_{i=1}^I \bigg(\frac{1}{\gamma_{i1}}\bigg)^{d_{i1+\alpha_\gamma+1}}\quad e^{-\big((\frac{\beta_\gamma}{\gamma_{i1}})+(\frac{c_{i1}}{\gamma_{i1}})^{d_{i1}}\big)}\times\\
&\times& \prod_{i=1}^I \prod_{j=2}^{n_i} \bigg(\frac{1}{\gamma_{ij}}\bigg)^{2d_{ij}+\alpha_\gamma+1}\quad e^{-\big((\frac{\beta_\gamma}{\gamma_{ij}})+(\frac{c_{ij}+c_{ij-1}}{\gamma_{ij}})^{d_{ij}}\big)}\Bigg)\times \\
&\times& \frac{\beta_0^{\alpha_0}}{\Gamma(\alpha_0)} \quad \beta_\gamma^{\alpha_0-1} e^{-\beta_\gamma\beta_0}
\end{eqnarray*}
\\
\\
\begin{eqnarray*}
&\propto& \Bigg(\prod_{i=1}^I e^{-\big(\frac{\beta_\gamma}{\gamma_{i1}}\big)}\prod_{i=1}^I \prod_{j=2}^{n_i} e^{-\big(\frac{\beta_\gamma}{\gamma_{ij}}\big)}\Bigg) \quad \beta_\gamma^{\alpha_0-1} e^{-\beta_\gamma\beta_0}\\
&=&e^{\{-\sum_{i=1}^I \sum_{j=1}^{n_i}\big(\frac{\beta_\gamma}{\gamma_{ij}}\big)\}}\quad \beta_\gamma^{\alpha_0-1} e^{-\beta_\gamma\beta_0}\\
&=& \beta_\gamma^{\alpha_0-1} e^{-\beta_\gamma\big(\beta_0+\sum_{i=1}^I \sum_{j=1}^{n_i}\big(\frac{\beta_\gamma}{\gamma_{ij}}\big))}\\
\\
&\propto& \beta_\gamma \sim Gamma\Bigg(\alpha_0,\beta_0+\sum_{i=1}^I \sum_{j=1}^{n_i}\big(\frac{\beta_\gamma}{\gamma_{ij}}\big)\Bigg)
\end{eqnarray*}
\\
\\
\\
\\
\chapter{Log-verosimilitudes}
\section{$ln(\pi(\alpha_d|(\theta_{ij})_{j=1}^{n_i}._{i=1}^I))$}
\begin{eqnarray*}
ln(\pi(\alpha_d|(\theta_{ij})_{j=1}^{n_i}._{i=1}^I)) &=& ln\Bigg(\Big(\frac{1}{\Gamma(\alpha_d+\alpha_\theta)}\Big)^I \Big(\frac{1}{\Gamma(2\alpha_d+\alpha_\theta)}\Big)^{\sum_{i=1}^I n_i} \quad \alpha_d^{\alpha_0-1} e^{-\alpha_d\beta_0} \times \\
&\times& \Bigg(\prod_{i=1}^I (d_{i1}+\beta_\theta)^{\alpha_d+\alpha_\theta} \quad \theta_{i1}^{\alpha_d+\alpha_\theta-1} \prod_{i=1}^I \prod_{j=2}^{n_i} (d_{ij}+d_{ij-1}+\beta_\theta)^{2\alpha_d+\alpha_\theta}\quad \theta_{ij}^{2\alpha_d+\alpha_\theta-1}\Bigg)\Bigg)
\end{eqnarray*}
\begin{eqnarray*}
&=& -I\times ln(\Gamma(\alpha_d+\alpha_\theta))-\sum_{i=1}^I n_i\times ln(\Gamma(2\alpha_d+\alpha_\theta))+(\alpha_0-1)\times ln(\alpha_d)-\alpha_d\beta_0 +\\
&+&\Bigg(\sum_{i=1}^I(\alpha_d+\alpha_\theta)\times ln(d_{i1}+\beta_\theta)+(\alpha_d+\alpha_\theta-1)\times ln(\theta_{i1})+\\
&+& \sum_{i=1}^I \sum_{j=2}^{n_i} (2\alpha_d+\alpha_\theta)\times ln(d_{ij}+d_{ij-1}+\beta_\theta)+(2\alpha_d+\alpha_\theta-1)\times ln(\theta_{ij})\Bigg)
\end{eqnarray*}
\\
\\
\section{$ln(\pi(\alpha_\theta|(\theta_{ij})_{i=1}^I._{j=1}^{n_i}))$}
\begin{eqnarray*}
ln(\pi(\alpha_\theta|(\theta_{ij})_{i=1}^I._{j=1}^{n_i})) &=&ln\Bigg(\Big(\frac{1}{\Gamma(\alpha_d+\alpha_\theta)}\Big)^I \Big(\frac{1}{\Gamma(2\alpha_d+\alpha_\theta)}\Big)^{\sum_{i=1}^I n_i} \quad \alpha_\theta^{\alpha_0-1} e^{-\alpha_\theta\beta_0} \times \\
&\times& \Bigg(\prod_{i=1}^I (d_{i1}+\beta_\theta)^{\alpha_d+\alpha_\theta} \quad \theta_{i1}^{\alpha_d+\alpha_\theta-1}\quad \prod_{i=1}^I \prod_{j=2}^{n_i} (d_{ij}+d_{ij-1}+\beta_\theta)^{2\alpha_d+\alpha_\theta} \quad \theta_{ij}^{2\alpha_d+\alpha_\theta-1}\Bigg)\Bigg)
\end{eqnarray*}
\begin{eqnarray*}
&=& -I\times ln(\Gamma(\alpha_d+\alpha_\theta))-\sum_{i=1}^I n_i\times ln(\Gamma(2\alpha_d+\alpha_\theta))+(\alpha_0-1)\times ln(\alpha_\theta)-\alpha_\theta\beta_0 +\\
&+&\Bigg(\sum_{i=1}^I(\alpha_d+\alpha_\theta)\times ln(d_{i1}+\beta_\theta)+(\alpha_d+\alpha_\theta-1)\times ln(\theta_{i1})+\\
&+& \sum_{i=1}^I \sum_{j=2}^{n_i} (2\alpha_d+\alpha_\theta)\times ln(d_{ij}+d_{ij-1}+\beta_\theta)+(2\alpha_d+\alpha_\theta-1)\times ln(\theta_{ij})\Bigg)
\end{eqnarray*}
\\
\\
\\
\section{$ln(\pi(\beta_\theta|(\theta_{ij})_{i=1}^I._{j=1}^{n_i}))$}
\begin{eqnarray*}
ln(\pi(\beta_\theta|(\theta_{ij})_{i=1}^I._{j=1}^{n_i})) &=& ln\Bigg( \Bigg(\prod_{i=1}^I (d_{i1}+\beta_\theta)^{\alpha_d+\alpha_\theta}\times\prod_{i=1}^I \prod_{j=2}^{n_i} (d_{ij}+d_{ij-1}+\beta_\theta)^{2\alpha_d+\alpha_\theta}\quad \Bigg)\times \\
&\times&\beta_\theta^{\alpha_0-1} e^{-\beta_\theta\big(\beta_0+\sum_{i=1}^I \sum_{j=1}^{n_i}\theta_{ij}\big)}\Bigg)
\end{eqnarray*}
\begin{eqnarray*}
&=&\sum_{i=1}^I (\alpha_d+\alpha_\theta)\times ln(d_{i1}+\beta_\theta)+\sum_{i=1}^I \sum_{j=2}^{n_i} ((2\alpha_d+\alpha_\theta)\times ln(d_{ij}+d_{ij-1}+\beta_\theta))+\\
&+&((\alpha_0-1)\times ln(\beta_\theta))-\beta_\theta\bigg(\beta_0+\sum_{i=1}^I \sum_{j=1}^{n_i} \theta_{ij}\bigg)
\end{eqnarray*}
\\
\\
\section{$ln(\pi(\alpha_\gamma|(\gamma_{ij})_{i=1}^I._{j=1}^{n_i}))$}
\begin{eqnarray*}
ln(\pi(\alpha_\gamma|(\gamma_{ij})_{i=1}^I._{j=1}^{n_i})) &=& ln\Bigg(\Bigg(\prod_{i=1}^I \prod_{j=1}^{n_i} \Big(\frac{1}{\gamma_{ij}}\Big)^{\alpha_\gamma}\Bigg) \quad \alpha_\gamma^{\alpha_0-1}e^{-\alpha_\gamma\beta_0}\Bigg)
\end{eqnarray*}
\begin{eqnarray*}
&=& -\sum_{i=1}^I \sum_{j=1}^{n_i} \big((\alpha_\gamma)\times ln(\gamma_{ij})\big)+\big((\alpha_0-1)\times ln(\alpha_\gamma)\big)-\alpha_\gamma\beta_0
\end{eqnarray*}
\\
\\
\\
\section{$ln(\pi(\beta_\gamma|(\gamma_{ij})_{i=1}^I._{j=1}^{n_i}))$}
\begin{eqnarray*}
ln(\pi(\beta_\gamma|(\gamma_{ij})_{i=1}^I._{j=1}^{n_i}))&=&ln\Bigg(\beta_\gamma^{\alpha_0-1} e^{-\beta_\gamma\big(\beta_0+\sum_{i=1}^I \sum_{j=1}^{n_i}\big(\frac{\beta_\gamma}{\gamma_{ij}}\big))}\Bigg)\\
&=&\Bigg((\alpha_0-1)\times ln(\beta_\gamma)\big)-\beta_\gamma\bigg(\beta_0+\sum_{i=1}^I \sum_{j=1}^{n_i}\big(\frac{\beta_\gamma}{\gamma_{ij}}\bigg)\Bigg)
\end{eqnarray*}
\end{document}